Interference example with cheats

hol/p4_concurrentScript.sml
@@ -14,13 +14,15 @@ open ottTheory;
 open pairTheory;
 open rich_listTheory;
 
+open p4_exec_semTheory p4_exec_sem_arch_soundnessTheory;
+
 val _ = new_theory "p4_concurrent";
 
 
 
-val trace_path_def = Define `
+Definition trace_path_def:
 trace_path R (n:num) init fin = NRC R (n:num) init fin
-`;
+End
 
 
 
@@ -67,7 +69,7 @@ QED
      
 
 
-Theorem arch_path_imples_conc:
+Theorem arch_path_implies_conc_thread1:
  ∀ n actx i io1 io2 a gsl framel status i' io1' io2' a' gsl' framel' status' thread2.
   trace_path ( \i f. arch_red actx i f) n ((i,io1,io2,a),gsl,framel,status) ((i',io1',io2',a'),gsl',framel',status') ⇒
   trace_path ( \i f. conc_red actx i f) n ((io1 ,io2 ,a ), ((i ,gsl ,framel ,status ) , thread2))
@@ -78,24 +80,74 @@ gvs[trace_path_def] >>
 REPEAT STRIP_TAC >> 
 gvs[NRC] >>
 PairCases_on ‘f’ >>
-
 Q.EXISTS_TAC ‘((f1,f2,f3),((f0,f4,f5,f6),thread2))’ >>
 CONJ_TAC >| [
+ SIMP_TAC list_ss [Once conc_red_cases]>>
+ DISJ1_TAC>>             
+ PairCases_on ‘thread2’ >>
+ PairCases_on ‘actx’ >>
+ srw_tac [] [clause_name_def],
 
-    SIMP_TAC list_ss [Once conc_red_cases]>>
-    DISJ1_TAC>>             
-    PairCases_on ‘thread2’ >>
-    PairCases_on ‘actx’ >>
-    srw_tac [][clause_name_def]
-    ,
-    RES_TAC >>    
-    FIRST_X_ASSUM (STRIP_ASSUME_TAC o (Q.SPECL [‘thread2’]))
-  ] 
-       
+ RES_TAC >>    
+ FIRST_X_ASSUM (STRIP_ASSUME_TAC o (Q.SPECL [‘thread2’]))
+]    
 QED
-     
 
-       
+Theorem arch_path_implies_conc_thread2:
+ ∀ n actx i io1 io2 a gsl framel status i' io1' io2' a' gsl' framel' status' thread1.
+  trace_path ( \i f. arch_red actx i f) n ((i,io1,io2,a),gsl,framel,status) ((i',io1',io2',a'),gsl',framel',status') ⇒
+  trace_path ( \i f. conc_red actx i f) n ((io1 ,io2 ,a ), (thread1, (i ,gsl ,framel ,status)))
+                                          ((io1',io2',a'), (thread1, (i',gsl',framel',status')))
+Proof
+Induct_on ‘n’ >>
+gvs[trace_path_def] >>
+REPEAT STRIP_TAC >> 
+gvs[NRC] >>
+PairCases_on ‘f’ >>
+Q.EXISTS_TAC ‘((f1,f2,f3),(thread1, (f0,f4,f5,f6)))’ >>
+CONJ_TAC >| [
+ SIMP_TAC list_ss [Once conc_red_cases]>>
+ DISJ2_TAC>>             
+ PairCases_on ‘thread1’ >>
+ PairCases_on ‘actx’ >>
+ srw_tac [] [clause_name_def],
+
+ RES_TAC >>    
+ FIRST_X_ASSUM (STRIP_ASSUME_TAC o (Q.SPECL [‘thread1’]))
+]    
+QED
+
+Theorem arch_exec_trace_1:
+!actx s s'.
+ arch_multi_exec actx s 1 = SOME s' ==>
+ trace_path ( \s s'. arch_red actx s s') 1 s s'
+Proof
+rpt strip_tac >>
+fs[arch_multi_exec_1, trace_path_def] >>
+PairCases_on ‘s’ >>
+ASSUME_TAC (ISPECL [“s5:arch_frame_list”, “alpha_dummy:'a itself”] arch_exec_sound_red) >>
+fs [arch_exec_sound]
+QED
+
+Theorem arch_exec_trace_n:
+!actx n s s'.
+ arch_multi_exec actx s n = SOME s' ==>
+ trace_path ( \s s'. arch_red actx s s') n s s'
+Proof
+Induct_on ‘n’ >| [
+ rpt strip_tac >>
+ PairCases_on ‘s’ >>
+ fs[arch_multi_exec_def, trace_path_def],
+
+ rpt strip_tac >>
+ subgoal ‘?s''. arch_multi_exec actx s n = SOME s'' /\
+                arch_multi_exec actx s'' 1 = SOME s'’ >- (
+  cheat
+ ) >>
+ metis_tac [arch_exec_trace_1, arch_paths_compose, arithmeticTheory.SUC_ONE_ADD]
+]
+QED
+
 
 
 val _ = export_theory ();
