hol/p4_from_json/concurrency_tests/concur1_interferenceScript.sml
@@ -1,0 +1,260 @@
+open HolKernel Parse bossLib boolSyntax;
+open p4_testLib p4_arch_auxTheory;
+open p4_concurrentTheory;
+
+val _ = new_theory "concur1_interleaving";
+
+(*
+(stmt_ass lval_null
+            (e_call (funn_inst "register")
+               [e_var (varn_name "r");
+                e_v
+                  (v_bit
+                     ([F; F; F; F; F; F; F; F; F; F; F; F; F; F; F; F; F; F;
+                       F; F; F; F; F; F; F; F; F; F; F; F; F; T],32));
+                e_v
+                  (v_bit
+                     ([ARB; ARB; ARB; ARB; ARB; ARB; ARB; ARB; ARB; ARB; ARB;
+                       ARB; ARB; ARB; ARB; ARB],16))]))
+*)
+
+val concur1_actx = ``([arch_block_inp;
+  arch_block_pbl "MyParser"
+    [e_var (varn_name "b"); e_var (varn_name "parsedHdr");
+     e_var (varn_name "meta"); e_var (varn_name "standard_metadata")];
+  arch_block_ffbl "postparser";
+  arch_block_pbl "MyVerifyChecksum"
+    [e_var (varn_name "hdr"); e_var (varn_name "meta")];
+  arch_block_pbl "MyIngress"
+    [e_var (varn_name "hdr"); e_var (varn_name "meta");
+     e_var (varn_name "standard_metadata")];
+  arch_block_pbl "MyEgress"
+    [e_var (varn_name "hdr"); e_var (varn_name "meta");
+     e_var (varn_name "standard_metadata")];
+  arch_block_pbl "MyComputeChecksum"
+    [e_var (varn_name "hdr"); e_var (varn_name "meta")];
+  arch_block_pbl "MyDeparser"
+    [e_var (varn_name "b"); e_var (varn_name "hdr")]; arch_block_out],
+ [("MyParser",
+   pblock_regular pbl_type_parser
+     [("MyParser",stmt_seq stmt_empty (stmt_trans (e_v (v_str "start"))),
+       [("packet",d_none); ("hdr",d_out); ("meta",d_inout);
+        ("standard_metadata",d_inout)])] []
+     [("start",stmt_seq stmt_empty (stmt_trans (e_v (v_str "accept"))))] []);
+  ("MyVerifyChecksum",
+   pblock_regular pbl_type_control
+     [("MyVerifyChecksum",stmt_seq stmt_empty stmt_empty,
+       [("hdr",d_inout); ("meta",d_inout)])] [] [] []);
+  ("MyIngress",
+   pblock_regular pbl_type_control
+     [("read_register",
+       stmt_seq
+         (stmt_seq
+            (stmt_ass lval_null
+               (e_call (funn_ext "register" "read")
+                  [e_var (varn_name "r"); e_var (varn_name "tmp");
+                   e_v
+                     (v_bit
+                        ([F; F; F; F; F; F; F; F; F; F; F; F; F; F; F; F; F;
+                          F; F; F; F; F; F; F; F; F; F; F; F; F; F; F],32))]))
+            (stmt_ass (lval_varname (varn_name "tmp"))
+               (e_binop (e_var (varn_name "tmp")) binop_add
+                  (e_v
+                     (v_bit
+                        ([F; F; F; F; F; F; F; F; F; F; F; F; F; F; F; T],16))))))
+         (stmt_ret (e_v v_bot)),[]);
+      ("write_register",
+       stmt_seq
+         (stmt_ass lval_null
+            (e_call (funn_ext "register" "write")
+               [e_var (varn_name "r");
+                e_v
+                  (v_bit
+                     ([F; F; F; F; F; F; F; F; F; F; F; F; F; F; F; F; F; F;
+                       F; F; F; F; F; F; F; F; F; F; F; F; F; F],32));
+                e_var (varn_name "tmp")])) (stmt_ret (e_v v_bot)),[]);
+      ("MyIngress",
+       stmt_seq
+         stmt_empty
+         (stmt_block []
+            (stmt_seq (stmt_app "flowlet" []) (stmt_app "new_flowlet" []))),
+       [("hdr",d_inout); ("meta",d_inout); ("standard_metadata",d_inout)])]
+     [(varn_name "tmp",tau_bit 16,NONE)] []
+     [("flowlet",[],"read_register",[]);
+      ("new_flowlet",[],"write_register",[])]);
+  ("MyEgress",
+   pblock_regular pbl_type_control
+     [("MyEgress",stmt_seq stmt_empty stmt_empty,
+       [("hdr",d_inout); ("meta",d_inout); ("standard_metadata",d_inout)])]
+     [] [] []);
+  ("MyComputeChecksum",
+   pblock_regular pbl_type_control
+     [("MyComputeChecksum",stmt_seq stmt_empty stmt_empty,
+       [("hdr",d_inout); ("meta",d_inout)])] [] [] []);
+  ("MyDeparser",
+   pblock_regular pbl_type_control
+     [("MyDeparser",stmt_seq stmt_empty stmt_empty,
+       [("packet",d_none); ("hdr",d_in)])] [] [] [])],
+ [("postparser",ffblock_ff v1model_postparser)],
+ v1model_input_f (v_struct [],v_struct []),v1model_output_f,
+ v1model_copyin_pbl,v1model_copyout_pbl,v1model_apply_table_f,
+ [("header",NONE,
+   [("isValid",[("this",d_in)],header_is_valid);
+    ("setValid",[("this",d_inout)],header_set_valid);
+    ("setInvalid",[("this",d_inout)],header_set_invalid)]);
+  ("",NONE,
+   [("mark_to_drop",[("standard_metadata",d_inout)],v1model_mark_to_drop);
+    ("verify",[("condition",d_in); ("err",d_in)],v1model_verify)]);
+  ("packet_in",NONE,
+   [("extract",[("this",d_in); ("headerLvalue",d_out)],
+     v1model_packet_in_extract);
+    ("lookahead",[("this",d_in); ("targ1",d_in)],v1model_packet_in_lookahead);
+    ("advance",[("this",d_in); ("bits",d_in)],v1model_packet_in_advance)]);
+  ("packet_out",NONE,
+   [("emit",[("this",d_in); ("data",d_in)],v1model_packet_out_emit)]);
+  ("register",
+   SOME
+     ([("this",d_out); ("size",d_none); ("targ1",d_in)],register_construct),
+   [("read",[("this",d_in); ("result",d_out); ("index",d_in)],register_read);
+    ("write",[("this",d_in); ("index",d_in); ("value",d_in)],register_write)])],
+ [("NoAction",stmt_seq stmt_empty (stmt_ret (e_v v_bot)),[])]):v1model_ascope actx``;
+
+val concur1_astate =
+ ``((0, (* Block index *)
+     [([T], 1)], (* Input list *)
+     [], (* Output list *)
+     (* 'a: *)
+     1, (* Number of extern objects *)
+     [(0, INR (v1model_v_ext_register [(fixwidth 16 [], 16)]))],
+     ["r", v_ext_ref 0],
+     [("flowlet",[]); ("new_flowlet",[])]), (* End of 'a env *)
+    [[(varn_name "r", (v_ext_ref 0, NONE))]], (* g_scope_list *)
+    arch_frame_list_empty, (* frame_list *)
+    status_running (* status *)
+   ):v1model_ascope astate``;
+
+val concur1_shared_s =
+ ``([([T], 1:num)], (* Input list *)
+    []: (bool list # num) list, (* Output list *)
+    (* 'a: *)
+    (1:num, (* Number of extern objects *)
+     [(0:num, INR (v1model_v_ext_register [(fixwidth 16 [], 16)]))]:(num # (core_v_ext + v1model_v_ext)) list,
+     ["r", v_ext_ref 0],
+     [("flowlet",[]:(e list # string # e list) list); ("new_flowlet",[])])
+   )``;
+
+val concur1_t1_s =
+ ``(0:num,
+    [[(varn_name "r", (v_ext_ref 0, NONE))]]:scope list,
+    arch_frame_list_empty,
+    status_running
+   )``;
+
+val concur1_t2_s =
+ ``(0:num,
+    [[(varn_name "r", (v_ext_ref 0, NONE))]]:scope list,
+    arch_frame_list_empty,
+    status_running
+   )``;
+
+Definition v1model_ascope_read_ext_obj_def:
+ v1model_ascope_read_ext_obj ((counter, ext_obj_map, v_map, ctrl):v1model_ascope) vname =
+  case ALOOKUP v_map vname of
+  | SOME (v_ext_ref n) =>
+   ALOOKUP ext_obj_map n
+  | _ => NONE
+End
+
+Definition v1model_ascope_of_conc_state_def:
+ v1model_ascope_of_conc_state (io1,io2,(ascope:v1model_ascope)) =
+  ascope
+End
+
+Definition p4_finished_def:
+ p4_finished ((io1 ,io2 , a), ((i1, gsl1, framel1, status1), (i2, gsl2, framel2, status2))) =
+  (io1 = [] /\ status1 = status_running /\ status2 = status_running)
+End
+
+(*
+(* 28 steps to finishing first function *)
+ val (_, ((i, _, in_out_list', _), _, arch_frame_list, status)) = debug_arch_from_step "v1model" concur1_actx concur1_astate 28
+
+(* 55 steps to finishing the entire program *)
+ val (_, ((i, _, in_out_list', _), _, arch_frame_list, status)) = debug_arch_from_step "v1model" concur1_actx concur1_astate 55
+
+First witness from
+  T1: 55 steps
+  T2: 55 steps
+
+Second witness from
+  T1: 28 steps
+  T2: 28 steps
+  T1: 27 steps
+  T2: 27 steps
+
+ val (_, ((i, _, in_out_list', _), g_scope_list, arch_frame_list, status)) = debug_arch_from_step "v1model" concur1_actx concur1_astate 55
+*)
+ val (_, ((i1', _, _, _), g_scope_list1', arch_frame_list1', status1')) = debug_arch_from_step "v1model" concur1_actx concur1_astate 55
+
+val t1_s' = “(0:num, ^g_scope_list1', arch_frame_list_empty, status_running)”;
+val t2_s' = “(0:num, ^g_scope_list1', arch_frame_list_empty, status_running)”;
+
+ val (_, ((_, io_list, io_list', ascope'), _, _, _)) = debug_arch_from_step "v1model" concur1_actx concur1_astate 55
+
+val shared_s' = “(^io_list, ^io_list', ^ascope')”;
+val shared_s'' =
+   “([]:(bool list # num) list,[([T],0:num)],3:num,
+     [(0:num,INR (v1model_v_ext_register [(w2v 2w,16)]));
+      (1,INL (core_v_ext_packet [])); (2,INL (core_v_ext_packet [T]))],
+     [("parseError",v_bit (w2v 0w,32)); ("b",v_ext_ref 1);
+      ("b_temp",v_ext_ref 2);
+      ("standard_metadata",
+       v_struct
+         [("ingress_port",v_bit (w2v 1w,9));
+          ("egress_spec",v_bit (w2v 0w,9)); ("egress_port",v_bit (w2v 0w,9));
+          ("instance_type",v_bit (w2v 0w,32));
+          ("packet_length",v_bit (w2v 0w,32));
+          ("enq_timestamp",v_bit (w2v 0w,32));
+          ("enq_qdepth",v_bit (w2v 0w,19));
+          ("deq_timedelta",v_bit (w2v 0w,32));
+          ("deq_qdepth",v_bit (w2v 0w,19));
+          ("ingress_global_timestamp",v_bit (w2v 0w,48));
+          ("egress_global_timestamp",v_bit (w2v 0w,48));
+          ("mcast_grp",v_bit (w2v 0w,16)); ("egress_rid",v_bit (w2v 0w,16));
+          ("checksum_error",v_bit (w2v 0w,1));
+          ("parser_error",v_bit (w2v 0w,32)); ("priority",v_bit (w2v 0w,3))]);
+      ("parsedHdr",v_struct []); ("hdr",v_struct []); ("meta",v_struct [])],
+     [("flowlet",[]:(e list # string # e list) list); ("new_flowlet",[])])”;
+
+(* TODO: You can be more specific about what differs in the two traces *)
+(* TODO: Fix t1_s, t2_s and shared_s to align with the concur1 example *)
+Theorem concur1_trace_path_interference:
+ ?n t1_s' t2_s' shared_s' shared_s''.
+  (trace_path ( \s s'. conc_red ^concur1_actx s s') n (^concur1_shared_s, (^concur1_t1_s, ^concur1_t2_s))
+                                            (shared_s', (t1_s', t2_s')) /\
+   p4_finished (shared_s', (t1_s', t2_s')) /\
+   v1model_ascope_read_ext_obj (v1model_ascope_of_conc_state shared_s') "r" =
+    SOME (INR (v1model_v_ext_register [(fixwidth 16 (n2v 1), 16)]))) /\
+  (trace_path ( \s s'. conc_red ^concur1_actx s s') n (^concur1_shared_s, (^concur1_t1_s, ^concur1_t2_s))
+                                            (shared_s'', (t1_s', t2_s')) /\
+   p4_finished (shared_s'', (t1_s', t2_s')) /\
+   v1model_ascope_read_ext_obj (v1model_ascope_of_conc_state shared_s') "r" =
+    SOME (INR (v1model_v_ext_register [(fixwidth 16 (n2v 2), 16)])))
+Proof
+EXISTS_TAC “55:num” >>
+EXISTS_TAC t1_s' >>
+EXISTS_TAC t2_s' >>
+EXISTS_TAC shared_s' >>
+EXISTS_TAC shared_s'' >>
+CONJ_TAC >| [
+ (* 1. For witness of r=1, t1 executes the first function, then t2 executes the first function, then t1 the rest, then t2 the rest. *)
+ cheat,
+
+ (* 2. For witness of r=2, use executable semantics, then arch_exec_trace_n,
+  * then arch_path_implies_conc_thread1, then executable semantics for thread 2, then
+  * arch_exec_trace_n, then arch_path_implies_conc_thread2, then conc_paths_compose. *)
+ cheat
+]
+QED
+
+val _ = export_theory ();
